more work... still doesn't verify

z-match.dfy
@@ -1,19 +1,44 @@
+/* Integer Predicates */
+
+predicate positive (i : int)
+{
+  1 <= i
+}
+
+predicate nonnegative (i : int)
+{
+  0 <= i
+}
+
 /* Array Predicates */
 
-predicate nonempty <T> (arr : array<T>)
+predicate nonnull <T> (arr : array<T>)
 {
-  arr != null && 0 < arr.Length
+  arr != null
+}
+
+predicate nonempty <T> (arr : array<T>)
+  requires nonnull(arr)
+{
+  0 < arr.Length
+}
+
+predicate contains <T(==)> (ele : T, arr : array<T>)
+  reads arr
+  requires nonnull(arr)
+{
+  exists idx :: 0 <= idx < arr.Length && arr[idx] == ele
 }
 
 predicate same_size <S, T> (arr1 : array<S>, arr2 : array<T>)
-  requires nonempty(arr1)
-  requires nonempty(arr2)
+  requires nonnull(arr1)
+  requires nonnull(arr2)
 {
   arr1.Length == arr2.Length
 }
 
 predicate valid_idx <T> (idx : int, arr : array<T>)
-  requires nonempty(arr)
+  requires nonnull(arr)
 {
   0 <= idx < arr.Length
 }
@@ -21,47 +46,70 @@ predicate valid_idx <T> (idx : int, arr : array<T>)
 /* NOTE: Maybe slices could be a record? Not worth it right now. */
 
 predicate valid_slice <T> (start : int, size : int, arr : array<T>)
-  requires nonempty(arr)
+  requires nonnull(arr)
 {
-  forall idx :: start <= idx < start + size ==> valid_idx(idx, arr)
+  size == 0 || (valid_idx(start, arr) && valid_idx(start + size - 1, arr))
 }
-/*
+
 predicate slice_eq <T(==)> (start1 : int, arr1 : array<T>, start2 : int, arr2 : array<T>, size : int)
   reads arr1
   reads arr2
-  requires nonempty(arr1)
-  requires nonempty(arr2)
-  requires valid_slice(start1, size, arr1)
-  requires valid_slice(start2, size, arr2)
+  requires nonnull(arr1)
+  requires nonnull(arr2)
 {
-  forall offset :: 0 <= offset < size ==> arr1[start1] == arr2[start2]
+  valid_slice(start1, size, arr1) &&
+  valid_slice(start2, size, arr2) &&
+  forall offset :: 0 <= offset < size ==> arr1[start1 + offset] == arr2[start2 + offset]
 }
-*/
+
 /* Z Predicates */
 
 predicate z_zero_correct (zs : array<int>)
   reads zs
+  requires nonnull(zs)
   requires nonempty(zs)
 {
   zs[0] == 0
 }
 
-predicate z_nonzero_correct(str : array<char>, zs : array<int>)
+predicate z_slices_valid (zs : array<int>)
+  reads zs
+  requires nonnull(zs)
+{
+  nonempty(zs) &&
+  forall idx :: 1 <= idx < zs.Length ==> valid_slice(idx, zs[idx], zs)
+}
+
+predicate z_nonzero_correct (str : array<char>, zs : array<int>)
   reads str
   reads zs
-  requires same_size(str, zs)
-  requires forall k :: 1 <= k < zs.Length ==> k + zs[k] <= zs.Length
+  requires nonnull(str)
+  requires nonnull(zs)
 {
-  forall idx :: 1 <= idx < zs.Length ==> forall k :: 0 <= k < zs[idx] ==> str[k] == str[idx + k]
+  forall idx :: 1 <= idx < zs.Length ==> slice_eq(0, str, idx, str, zs[idx])
+}
+
+predicate z_correct (str : array<char>, zs : array<int>)
+  reads str
+  reads zs
+  requires nonnull(str)
+  requires nonnull(zs)
+  requires nonempty(str)
+  requires nonempty(zs)
+  requires same_size(str, zs)
+{
+  z_zero_correct(zs) &&
+  z_slices_valid(zs) &&
+  z_nonzero_correct(str, zs)
 }
 
 method z_algorithm_naive(str : array<char>) returns (zs : array<int>)
+  requires nonnull(str)
   requires nonempty(str)
 
+  ensures nonnull(zs)
   ensures same_size(str, zs)
-  ensures z_zero_correct(zs)
-  ensures forall k :: 1 <= k < zs.Length ==> k + zs[k] <= zs.Length // TODO: Add Z's sanity check predicate
-  ensures z_nonzero_correct(str, zs)
+  ensures z_correct(str, zs)
 { // TODO: Refactor invariants as predicates
   zs := new int[str.Length];
 
@@ -72,14 +120,13 @@ method z_algorithm_naive(str : array<char>) returns (zs : array<int>)
   while (i < zs.Length)
     invariant 1 <= i <= zs.Length
     invariant z_zero_correct(zs)
-    invariant forall k :: 1 <= k < i ==> k + zs[k] <= zs.Length
-    invariant forall k :: 1 <= k < i ==> forall l :: 0 <= l < zs[k] ==> str[l] == str[k + l]
+    invariant forall k :: 1 <= k < i ==> slice_eq(0, str, k, str, zs[k])
   {
     var j := 0;
 
     while (j < zs.Length - i)
       invariant 0 <= j <= zs.Length - i
-      invariant forall k :: 0 <= k < j ==> str[k] == str[i + k]
+      invariant slice_eq(0, str, i, str, j)
     {
       if str[j] != str[i + j] {
         break;
@@ -95,11 +142,12 @@ method z_algorithm_naive(str : array<char>) returns (zs : array<int>)
 }
 
 method z_algorithm(str : array<char>) returns (zs : array<int>)
+  requires nonnull(str)
   requires nonempty(str)
+
+  ensures nonnull(zs)
   ensures same_size(str, zs)
-  ensures z_zero_correct(zs)
-  ensures forall k :: 1 <= k < zs.Length ==> k + zs[k] <= zs.Length // TODO: Add Z's sanity check predicate
-  ensures z_nonzero_correct(str, zs)
+  ensures z_correct(str, zs)
 {
   zs := new int[str.Length];
   zs[0] := 0;
@@ -111,10 +159,10 @@ method z_algorithm(str : array<char>) returns (zs : array<int>)
     invariant 1 <= i <= zs.Length
     invariant z_zero_correct(zs)
     invariant j < i
-    invariant forall k :: 1 <= k < i ==> k + zs[k] <= zs.Length
+    invariant forall k :: 1 <= k < i ==> valid_slice(k, zs[k], zs)
     invariant j+zs[j] == maxZ
     invariant maxZ <= zs.Length
-    invariant forall k :: 1 <= k < i ==> forall l :: 0 <= l < zs[k] ==> str[l] == str[k + l]
+    invariant forall k :: 1 <= k < i ==> slice_eq(0, str, k, str, zs[k])
   {
     if (maxZ < i){
       var l := 0;
@@ -122,13 +170,13 @@ method z_algorithm(str : array<char>) returns (zs : array<int>)
       
       while (i+l<str.Length) && (str[i+l]==str[l])
         invariant 1 <= i+l <= str.Length
-        invariant forall k :: 1 <= k < i ==> k + zs[k] <= zs.Length
+        invariant forall k :: 1 <= k < i ==> valid_slice(k, zs[k], zs)
         invariant i+zs[i] <= zs.Length
         invariant zs[i] == l
         invariant z_zero_correct(zs)
         invariant maxZ <= zs.Length
-        invariant forall k :: 1 <= k < i ==> forall l :: 0 <= l < zs[k] ==> str[l] == str[k + l]
-        invariant forall m :: 0 <= m < zs[i] ==> str[m] == str[i+m]
+        invariant forall k :: 1 <= k < i ==> slice_eq(0, str, k, str, zs[k])
+        invariant slice_eq(0, str, i, str, zs[i])
       {
         zs[i] := zs[i]+1;
         l := l+1;  
@@ -151,12 +199,12 @@ method z_algorithm(str : array<char>) returns (zs : array<int>)
         while (i+l<str.Length) && (str[i+l]==str[l])
             invariant 1 <= i <= zs.Length
             invariant z_zero_correct(zs)
-            invariant forall k :: 1 <= k < i ==> k + zs[k] <= zs.Length
+            invariant forall k :: 1 <= k < i ==> valid_slice(k, zs[k], zs)
             invariant maxZ <= zs.Length
             invariant i+zs[i] <= zs.Length
             invariant zs[i] == l
-            invariant forall k :: 1 <= k < i ==> forall l :: 0 <= l < zs[k] ==> str[l] == str[k + l]
-            invariant forall m :: 0 <= m < zs[i] ==> str[m] == str[i+m]
+            invariant forall k :: 1 <= k < i ==> slice_eq(0, str, k, str, zs[k])
+            invariant slice_eq(0, str, i, str, zs[i])
         {
           zs[i] := zs[i]+1;
           l := l+1;
@@ -170,11 +218,17 @@ method z_algorithm(str : array<char>) returns (zs : array<int>)
 }
 
 method print_arr <T> (arr : array<T>)
-  requires nonempty(arr)
+  requires nonnull(arr)
 {
   var i := 0;
 
   print "[";
+
+  if (arr.Length == 0)
+  {
+    print "[]";
+    return;
+  }
 
   while (i < arr.Length - 1)
     invariant 0 <= i <= arr.Length - 1
@@ -192,13 +246,18 @@ method print_arr <T> (arr : array<T>)
 method array_of_string (str : string) returns (ret : array<char>)
   requires 0 < |str|
 
+  ensures nonnull(ret)
   ensures nonempty(ret)
+  ensures |str| == ret.Length
+  ensures forall idx :: 0 <= idx < |str| ==> str[idx] == ret[idx]
 {
   ret := new char[|str|];
 
   var i := 0;
 
   while (i < |str|)
+  invariant 0 <= i <= |str|
+  invariant forall k :: 0 <= k < i ==> str[k] == ret[k]
   {
     ret[i] := str[i];
 
@@ -206,10 +265,80 @@ method array_of_string (str : string) returns (ret : array<char>)
   }
 }
 
+method matches(pattern : array<char>, text : array<char>) returns (ret : int)
+  requires nonnull(pattern)
+  requires nonnull(text)
+  requires !contains('$', pattern)
+  requires !contains('$', text)
+
+  //ensures (ret != -1 && slice_eq(0, pattern, ret, text, pattern.Length)) || (ret == -1 && forall idx :: 0 <= idx < text.Length ==> !slice_eq(0, pattern, idx, text, pattern.Length))
+{
+
+  ret := -1;
+
+  var conc := new char[pattern.Length + text.Length + 1];
+
+  var i := 0;
+
+  while (i < conc.Length)
+  invariant 0 <= i <= conc.Length
+  invariant forall k :: 0 <= k < i ==> if k < pattern.Length then conc[k] == pattern[k] else if k == pattern.Length then conc[k] == '$' else conc[k] == text[k - (pattern.Length + 1)]
+  invariant forall k :: 0 <= k < i ==> if k < pattern.Length then slice_eq(0, pattern, 0, conc, k) else if k == pattern.Length then conc[k] == '$' else slice_eq(0, text, pattern.Length + 1, conc, k - (pattern.Length + 1))
+  {
+    if (i < pattern.Length) {
+      conc[i] := pattern[i];
+    } else if (i == pattern.Length) {
+      conc[i] := '$';
+    } else {
+      conc[i] := text[i - (pattern.Length + 1)];
+    }
+
+    i := i + 1;
+  }
+
+  print_arr(conc);
+
+  //assert(slice_eq(0, pattern, 0, conc, pattern.Length));
+  //assert(slice_eq(0, text, pattern.Length + 1, conc, text.Length));
+
+  var zs := z_algorithm(conc);
+
+  // assert(forall idx :: 0 <= idx < zs.Length ==> zs[idx] <= pattern.Length);
+
+  // assert (forall idx :: 0 <= idx < conc.Length ==> if zs[idx] == pattern.Length then slice_eq(0, conc, idx, conc, pattern.Length) else true);
+  // assert (forall idx :: 0 <= idx < conc.Length ==> if slice_eq(0, conc, idx, conc, pattern.Length) then slice_eq(0, pattern, idx - (pattern.Length + 1), text, pattern.Length) else true);
+  //assert (forall idx :: pattern.Length + 1 <= idx < conc.Length ==> if zs[idx] == pattern.Length then slice_eq(0, pattern, idx - (pattern.Length + 1), text, pattern.Length) else true);
+
+  print_arr(zs);
+
+  i := pattern.Length + 1;
+
+  while (i < conc.Length)
+    invariant pattern.Length + 1 <= i <= conc.Length
+    //invariant ret == -1 || slice_eq(0, pattern, ret, text, pattern.Length)
+    //invariant ret != -1 ==> slice_eq(0, pattern, ret, text, pattern.Length)
+    //invariant ret == -1 ==> (forall k :: pattern.Length + 1 <= k < i ==> zs[k] < pattern.Length)
+    //invariant ret == -1 ==> (forall k :: pattern.Length + 1 <= k < i ==> !slice_eq(0, pattern, k - (pattern.Length + 1), text, pattern.Length))
+    //invariant (ret != -1 && slice_eq(0, pattern, ret, text, pattern.Length)) || (ret == -1 && forall k :: pattern.Length + 1 <= k < i ==> !slice_eq(0, pattern, k - (pattern.Length + 1), text, pattern.Length))
+    // invariant b ==> exists idx :: 0 <= idx < i && slice_eq(0, pattern, idx - (pattern.Length + 1), text, pattern.Length)
+  {
+    if (zs[i] >= pattern.Length) {
+      ret := i - (pattern.Length + 1);
+      break;
+    }
+
+    i := i + 1;
+  }
+}
+
 method Main() {
-  var str := "heheh";
-  var str_as_arr := array_of_string(str);
-  print_arr(str_as_arr);
-  var res := z_algorithm(str_as_arr);
-  print_arr(res);
+  var pattern := "ana";
+  var text := "banana";
+
+  var pattern' := array_of_string(pattern);
+  var text' := array_of_string(text);
+
+  var b := matches(pattern', text');
+  print b;
+  print "\n";
 }
